LeanSAT/LRAT/Internal.lean
@@ -3,6 +3,7 @@ Copyright (c) 2024 Lean FRO, LLC. All rights reserved.
 Released under Apache 2.0 license as described in the file LICENSE.
 Authors: Henrik Böving
 -/
+import LeanSAT.LRAT.Internal.Actions
 import LeanSAT.LRAT.Internal.Assignment
 import LeanSAT.LRAT.Internal.CNF
 import LeanSAT.LRAT.Internal.Formula
